$\dfrac{x + 2}{x} > 0$

$x + 2 > 0 \rightarrow x > -2$

$x > 0 \rightarrow x > 0$

||-2||0||
|-|-|-|-|-|
|-|+|+|+|+|
|-|-|-|+|+|
|=|=|=|=|=|
|+|-|-|+|+|

Risultato: $x < -2 \lor x > 0$

---

$\dfrac{1}{x - 1} + \dfrac{x}{x + 1} \ge 2$

CE: $x \neq 1 \land x \neq -1$

$\dfrac{(x + 1) + (x (x - 1))}{x^2 - 1} \ge 2$

$\dfrac{(x + 1) + (x (x - 1)) - 2 (x^2 - 1)}{x^2 - 1} \ge 0$

Studiamo il segno:

Denominatore:

$x^2 - 1 \ge 0 \rightarrow x^2 \ge 1 \rightarrow x \le -1 \lor x \ge 1$

Numeratore:

$(x + 1) + (x (x - 1)) - 2 (x^2 - 1) \ge 0$

$x + 1 + x^2 - x - 2x^2 - 2 \ge 0$

$- x^2 - 1 \ge 0$

$x^2 \le -1 \rightarrow \not\exist x \in \mathbb{R}$

Tabella:

||-1||1||
|-|-|-|-|-|
|+|+|-|+|+|
|=|=|=|=|=|
|+|+|-|+|+|