$\lim\limits_{x \rightarrow 0} \dfrac{\log (1 + x^2)}{\sqrt{x + 1} - 1}$

$\lim\limits_{x \rightarrow 0} \dfrac{\log (1 + 0)}{\sqrt{0 + 1} - 1} = \dfrac{0}{0}$

Numeratore:

$\dfrac{d}{dx} \log (1 + x^2) =$

$= \dfrac{1}{x^2 + 1} \cdot \dfrac{d}{dx} (x^2 + 1) =$

$= \dfrac{2x}{x^2 + 1}$

Denominatore:

$\dfrac{d}{dx} \sqrt{x + 1} - 1 =$

$= \dfrac{d}{dx} (\sqrt{x + 1}) =$

$= \dfrac{1}{2} (x + 1)^{- \dfrac{1}{2}} =$

$= \dfrac{1}{2 \sqrt{x + 1}}$

Ricalcoliamo il limite:

$\lim \limits_{x \rightarrow 0} \dfrac{2x}{x^2 + 1} \cdot 2 \sqrt{x + 1} =$

$= \dfrac{4x \sqrt{x + 1}}{x^2 + 1} =$

$= \dfrac{4 \cdot 0 \sqrt{0 + 1}}{0^2 + 1} =$

$= \dfrac{0}{1} = 0$
